SigmaCalculus is now self-contained and does not depend on Closed

pcuic/theories/PCUICSigmaCalculus.v
@@ -1,8 +1,7 @@
 From Coq Require Import Morphisms.
 From MetaCoq.Template Require Import config utils.
 From MetaCoq.PCUIC Require Import PCUICAst PCUICAstUtils PCUICCases PCUICInduction
-  PCUICLiftSubst PCUICUnivSubst
-  PCUICTyping PCUICClosed PCUICEquality PCUICWeakeningEnv.
+  PCUICLiftSubst PCUICUnivSubst.
 
 Require Import ssreflect ssrbool.
 From Equations Require Import Equations.
@@ -13,16 +12,1019 @@ Set Default Goal Selector "!".
 
 (** * Theory of σ-calculus operations *)
 
-Open Scope sigma_scope.
+Declare Scope sigma_scope.
+Delimit Scope sigma_scope with sigma.
+Local Open Scope sigma_scope.
+Ltac sigma := autorewrite with sigma.
+Tactic Notation "sigma" "in" hyp(id) := autorewrite with sigma in id.
 
-Hint Rewrite @lift_rename Nat.add_0_r : sigma.
-Hint Rewrite @subst_consn_nil @subst_consn_tip : sigma.
-Hint Rewrite idsn_length : len.
+Definition substitution := nat -> term.
+Bind Scope sigma_scope with substitution.
+
+Hint Rewrite Nat.add_0_r : sigma.
+
+Ltac nat_compare_specs :=
+  match goal with
+  | |- context [?x <=? ?y] =>
+    destruct (Nat.leb_spec x y); try lia
+  | |- context [?x <? ?y] =>
+    destruct (Nat.ltb_spec x y); try lia
+  end.
+
+(* Sigma calculus*)
+
+Lemma shiftn_ext n f f' : (forall i, f i = f' i) -> forall t, shiftn n f t = shiftn n f' t.
+Proof.
+  intros.
+  unfold shiftn. destruct Nat.ltb; congruence.
+Qed.
+
+Instance shiftn_proper : Proper (Logic.eq ==> `=1` ==> `=1`) shiftn.
+Proof.
+  intros x y -> f g Hfg ?. now apply shiftn_ext.
+Qed.
+
+Lemma rename_ext f f' : (forall i, f i = f' i) -> (forall t, rename f t = rename f' t).
+Proof.
+  intros. revert f f' H.
+  elim t using term_forall_list_ind; simpl in |- *; intros; try easy ;
+    try (try rewrite H; try rewrite H0 ; try rewrite H1 ; easy);
+    try solve [f_equal; solve_all; eauto using shiftn_ext].
+  - f_equal; solve_all.
+    * now apply e, shiftn_ext.
+    * apply map_branch_eq_spec; solve_all; eauto using shiftn_ext.
+  - f_equal; auto. red in X. solve_all.
+    eapply map_def_eq_spec; auto. now apply b, shiftn_ext.
+  - f_equal; auto. red in X. solve_all.
+    eapply map_def_eq_spec; auto. now apply b, shiftn_ext.
+Qed.
+
+Instance rename_proper : Proper (`=1` ==> Logic.eq ==> Logic.eq) rename.
+Proof. intros f f' Hff' t t' ->. now apply rename_ext. Qed.
+
+Instance rename_proper_pointwise : Proper (`=1` ==> pointwise_relation _ Logic.eq) rename.
+Proof. intros f f' Hff' t. now apply rename_ext. Qed.
+
+
+Definition lift_renaming n k :=
+  fun i =>
+    if Nat.leb k i then (* Lifted *) n + i
+    else i.
+
+Lemma shiftn_lift_renaming n m k :
+  shiftn m (lift_renaming n k) =1 lift_renaming n (m + k).
+Proof.
+  unfold lift_renaming, shiftn. intros i.
+  repeat (nat_compare_specs; try lia).
+Qed.
+
+Lemma lift_rename n k t : lift n k t = rename (lift_renaming n k) t.
+Proof.
+  revert n k.
+  elim t using term_forall_list_ind; simpl in |- *; intros; try reflexivity;
+    try (rewrite ?H ?H0 ?H1; reflexivity);
+    try solve [f_equal; solve_all].
+  - f_equal; eauto.
+    now rewrite H0 shiftn_lift_renaming.
+  - f_equal; eauto.
+    now rewrite H0 shiftn_lift_renaming.
+  - f_equal; eauto.
+    rewrite H1. now rewrite shiftn_lift_renaming.
+  - f_equal; auto.
+    * solve_all. now rewrite e shiftn_lift_renaming.
+    * solve_all. apply map_branch_eq_spec. now rewrite H0 shiftn_lift_renaming.
+  - f_equal; auto.
+    red in X. solve_all. apply map_def_eq_spec; auto.
+    rewrite b. now rewrite shiftn_lift_renaming.
+  - f_equal; auto.
+    red in X. solve_all. apply map_def_eq_spec; auto.
+    rewrite b. now rewrite shiftn_lift_renaming.
+Qed.
+Hint Rewrite @lift_rename : sigma.
+
+Definition up k (s : nat -> term) :=
+  fun i =>
+    if k <=? i then rename (Nat.add k) (s (i - k))
+    else tRel i.
+
+Lemma shiftn_compose n f f' : shiftn n f ∘ shiftn n f' =1 shiftn n (f ∘ f').
+Proof.
+  unfold shiftn. intros x.
+  elim (Nat.ltb_spec x n) => H.
+  - now rewrite (proj2 (Nat.ltb_lt x n)).
+  - destruct (Nat.ltb_spec (n + f' (x - n)) n).
+    * lia.
+    * assert (n + f' (x - n) - n = f' (x - n)) as ->; lia.
+Qed.
+
+Lemma map_branches_shiftn (fn : (nat -> nat) -> term -> term) f f' l : 
+  map_branches_shift fn f (map_branches_shift fn f' l) = 
+  List.map (fun i => map_branch (fn (shiftn #|bcontext i| f) ∘ (fn (shiftn #|bcontext i| f'))) i) l.
+Proof.
+  rewrite map_map_compose. apply map_ext => i.
+  rewrite map_branch_map_branch.
+  simpl. now apply map_branch_eq_spec.
+Qed.
+
+Lemma rename_compose f f' : rename f ∘ rename f' =1 rename (f ∘ f').
+Proof.
+  intros x.
+  induction x in f, f' |- * using term_forall_list_ind; simpl; 
+    rewrite ?map_branch_map_branch ?map_predicate_map_predicate;
+    f_equal;
+    auto; solve_all.
+
+  - rewrite map_map_compose. apply All_map_eq. solve_all.
+  - rewrite IHx2. apply rename_ext, shiftn_compose.
+  - rewrite IHx2. apply rename_ext, shiftn_compose.
+  - rewrite IHx3. apply rename_ext, shiftn_compose.
+  - rewrite /rename_predicate map_predicate_map_predicate.
+    solve_all; len. rewrite e.
+    apply rename_ext, shiftn_compose. 
+  - rewrite map_branches_shiftn. solve_all. apply map_branch_eq_spec.
+    rewrite H. apply rename_ext, shiftn_compose.
+  - rewrite map_map_compose; apply All_map_eq. solve_all.
+    rewrite map_def_map_def map_length.
+    apply map_def_eq_spec; auto.
+    rewrite b. apply rename_ext, shiftn_compose.
+  - rewrite map_map_compose; apply All_map_eq. solve_all.
+    rewrite map_def_map_def map_length.
+    apply map_def_eq_spec; auto.
+    rewrite b. apply rename_ext, shiftn_compose.
+Qed.
+
+Lemma up_up k k' s : up k (up k' s) =1 up (k + k') s.
+Proof.
+  red. intros x. unfold up.
+  elim (Nat.leb_spec k x) => H.
+  - elim (Nat.leb_spec (k + k') x) => H'.
+    + elim (Nat.leb_spec k' (x - k)) => H''.
+      ++ rewrite Nat.sub_add_distr.
+         rewrite -> rename_compose. apply rename_ext. intros. lia.
+      ++ simpl. lia.
+    + edestruct (Nat.leb_spec k' (x - k)); simpl; lia_f_equal.
+  - elim (Nat.leb_spec (k + k') x) => H'; lia_f_equal.
+Qed.
+
+Fixpoint inst s u :=
+  match u with
+  | tRel n => s n
+  | tEvar ev args => tEvar ev (List.map (inst s) args)
+  | tLambda na T M => tLambda na (inst s T) (inst (up 1 s) M)
+  | tApp u v => tApp (inst s u) (inst s v)
+  | tProd na A B => tProd na (inst s A) (inst (up 1 s) B)
+  | tLetIn na b ty b' => tLetIn na (inst s b) (inst s ty) (inst (up 1 s) b')
+  | tCase ind p c brs =>
+    let p' := map_predicate id (inst s) (inst (up #|p.(pcontext)| s)) p in
+    let brs' := map (fun br => map_branch (inst (up #|br.(bcontext)| s)) br) brs in
+    tCase ind p' (inst s c) brs'
+  | tProj p c => tProj p (inst s c)
+  | tFix mfix idx =>
+    let mfix' := map (map_def (inst s) (inst (up (List.length mfix) s))) mfix in
+    tFix mfix' idx
+  | tCoFix mfix idx =>
+    let mfix' := map (map_def (inst s) (inst (up (List.length mfix) s))) mfix in
+    tCoFix mfix' idx
+  | x => x
+  end.
+
+Definition subst_fn (l : list term) :=
+  fun i =>
+    match List.nth_error l i with
+    | None => tRel (i - List.length l)
+    | Some t => t
+    end.
+
+Lemma up_ext k s s' : s =1 s' -> up k s =1 up k s'.
+Proof.
+  unfold up. intros Hs t. elim (Nat.leb_spec k t) => H; auto.
+  f_equal. apply Hs.
+Qed.
+
+Lemma inst_ext s s' : s =1 s' -> inst s =1 inst s'.
+Proof.
+  intros Hs t. revert s s' Hs.
+  elim t using term_forall_list_ind; simpl in |- *; intros; try easy ;
+    try (try rewrite H; try rewrite H0 ; try rewrite H1 ; easy);
+    try solve [f_equal; solve_all; eauto using up_ext].
+  - f_equal; solve_all.
+    * now apply e, up_ext.
+    * apply map_branch_eq_spec; solve_all; eauto using up_ext.
+  - f_equal; eauto. red in X. solve_all.
+    apply map_def_eq_spec; auto. now apply b, up_ext.
+  - f_equal; eauto. red in X. solve_all.
+    apply map_def_eq_spec; auto. now apply b, up_ext.
+Qed.
+
+Instance proper_inst : Proper (`=1` ==> Logic.eq ==> Logic.eq) inst.
+Proof.
+  intros f f' Hff' t t' ->. now apply inst_ext.
+Qed.
+
+Instance proper_inst' : Proper (`=1` ==> pointwise_relation _ Logic.eq) inst.
+Proof.
+  intros f f' Hff' t. now apply inst_ext.
+Qed.
+
+Instance up_proper k : Proper (`=1` ==> `=1`) (up k).
+Proof. reduce_goal. now apply up_ext. Qed.
+
+Definition ren (f : nat -> nat) : nat -> term :=
+  fun i => tRel (f i).
 
 Instance ren_ext : Morphisms.Proper (`=1` ==> `=1`)%signature ren.
 Proof.
   reduce_goal. unfold ren. now rewrite H.
 Qed.
+  
+Lemma ren_shiftn n f : up n (ren f) =1 ren (shiftn n f).
+Proof.
+  unfold ren, up, shiftn.
+  intros i.
+  elim (Nat.ltb_spec i n) => H; elim (Nat.leb_spec n i) => H'; try lia; trivial.
+Qed.
+
+Lemma rename_inst f : rename f =1 inst (ren f).
+Proof.
+  intros t. revert f.
+  elim t using term_forall_list_ind; simpl in |- *; intros; try easy ;
+    try (try rewrite H; try rewrite H0 ; try rewrite H1 ; easy);
+    try solve [f_equal; solve_all].
+
+  - f_equal; eauto. now rewrite H0 -ren_shiftn.
+  - f_equal; eauto. now rewrite H0 -ren_shiftn.
+  - f_equal; eauto. now rewrite H1 -ren_shiftn.
+  - f_equal; eauto; solve_all.
+    * now rewrite e -ren_shiftn.
+    * apply map_branch_eq_spec. now rewrite H0 -ren_shiftn.
+  - f_equal; eauto. solve_all. apply map_def_eq_spec; auto.
+    now rewrite b ren_shiftn.
+  - f_equal; eauto. solve_all. apply map_def_eq_spec; auto.
+    now rewrite b ren_shiftn.
+Qed.
+
+Hint Rewrite @rename_inst : sigma.
+
+(** Show the σ-calculus equations.
+
+    Additional combinators: [idsn n] for n-identity, [consn] for consing a parallel substitution.
+ *)
+
+Notation "t '.[' σ ]" := (inst σ t) (at level 6, format "t .[ σ ]") : sigma_scope.
+
+Definition subst_cons (t : term) (f : nat -> term) :=
+  fun i =>
+    match i with
+    | 0 => t
+    | S n => f n
+    end.
+
+Notation " t ⋅ s " := (subst_cons t s) (at level 70) : sigma_scope.
+
+Instance subst_cons_proper : Proper (Logic.eq ==> `=1` ==> `=1`) subst_cons.
+Proof. intros x y -> f f' Hff'. intros i. destruct i; simpl; trivial. Qed.
+
+Definition shift : nat -> term := tRel ∘ S.
+Notation "↑" := shift : sigma_scope.
+
+Definition subst_compose (σ τ : nat -> term) :=
+  fun i => (σ i).[τ].
+
+Infix "∘s" := subst_compose (at level 40) : sigma_scope.
+
+Instance subst_compose_proper : Proper (`=1` ==> `=1` ==> `=1`) subst_compose.
+Proof.
+  intros f f' Hff' g g' Hgg'. intros x. unfold subst_compose.
+  now rewrite Hgg' Hff'.
+Qed.
+
+Definition Up σ : substitution := tRel 0 ⋅ (σ ∘s ↑).
+Notation "⇑ s" := (Up s) (at level 20).
+
+Instance Up_ext : Proper (`=1` ==> `=1`) Up.
+Proof.
+  unfold Up. reduce_goal. unfold subst_compose, subst_cons.
+  destruct a => //. now rewrite H.
+Qed.
+
+Lemma up_Up σ : up 1 σ =1 ⇑ σ.
+Proof.
+  unfold up.
+  intros i.
+  elim (Nat.leb_spec 1 i) => H.
+  - unfold subst_cons, shift. destruct i.
+    -- lia.
+    -- simpl. rewrite Nat.sub_0_r.
+       unfold subst_compose.
+       now rewrite rename_inst.
+  - red in H. destruct i; [|lia]. reflexivity.
+Qed.
+
+(** Simplify away [up 1] *)
+Hint Rewrite up_Up : sigma.
+
+Definition ids (x : nat) := tRel x.
+
+Definition ren_id (x : nat) := x.
+
+Lemma ren_id_ids : ren ren_id =1 ids.
+Proof. reflexivity. Qed.
+
+Lemma shiftn_id n : shiftn n ren_id =1 ren_id.
+Proof.
+  intros i; unfold shiftn.
+  elim (Nat.ltb_spec i n) => H //.
+  unfold ren_id. lia.
+Qed.
+
+Lemma rename_ren_id : rename ren_id =1 id.
+Proof.
+  intros t. unfold id.
+  elim t using term_forall_list_ind; simpl in |- *; intros; try easy ;
+    try (try rewrite H; try rewrite H0 ; try rewrite H1 ; easy);
+    try solve [f_equal; solve_all].
+
+  - f_equal; auto. now rewrite shiftn_id.
+  - f_equal; auto. now rewrite shiftn_id.
+  - f_equal; auto. now rewrite shiftn_id.
+  - setoid_rewrite shiftn_id. f_equal; solve_all. 
+    now rewrite shiftn_id.
+  - f_equal; auto. solve_all.
+    apply map_def_id_spec; auto.
+    now rewrite shiftn_id.
+  - f_equal; auto. solve_all.
+    apply map_def_id_spec; auto.
+    now rewrite shiftn_id.
+Qed.
+
+Lemma subst_ids t : t.[ids] = t.
+Proof.
+  now rewrite -ren_id_ids -rename_inst rename_ren_id.
+Qed.
+
+Hint Rewrite subst_ids : sigma.
+
+Lemma compose_ids_r σ : σ ∘s ids =1 σ.
+Proof.
+  unfold subst_compose. intros i; apply subst_ids.
+Qed.
+
+Lemma compose_ids_l σ : ids ∘s σ =1 σ.
+Proof. reflexivity. Qed.
+
+Hint Rewrite compose_ids_r compose_ids_l : sigma.
+
+Definition shiftk (k : nat) (x : nat) := tRel (k + x).
+Notation "↑^ k" := (shiftk k) (at level 30, k at level 2, format "↑^ k") : sigma_scope.
+
+Lemma shiftk_0 : shiftk 0 =1 ids.
+Proof.
+  intros i. reflexivity.
+Qed.
+
+Definition subst_consn {A} (l : list A) (σ : nat -> A) :=
+  fun i =>
+    match List.nth_error l i with
+    | None => σ (i - List.length l)
+    | Some t => t
+    end.
+
+Notation " t ⋅n s " := (subst_consn t s) (at level 40) : sigma_scope.
+
+Lemma subst_consn_nil {A} (σ : nat -> A) : nil ⋅n σ =1 σ.
+Proof.
+  intros i. unfold subst_consn. rewrite nth_error_nil.
+  now rewrite Nat.sub_0_r.
+Qed.
+Hint Rewrite @subst_consn_nil : sigma.
+
+Lemma subst_consn_subst_cons t l σ : (t :: l) ⋅n σ =1 (t ⋅ subst_consn l σ).
+Proof.
+  intros i. unfold subst_consn. induction i; simpl; trivial.
+Qed.
+
+Lemma subst_consn_tip t σ : [t] ⋅n σ =1 (t ⋅ σ).
+Proof. now rewrite subst_consn_subst_cons subst_consn_nil. Qed.
+Hint Rewrite @subst_consn_tip : sigma.
+
+Instance subst_consn_proper {A} : Proper (Logic.eq ==> `=1` ==> `=1`) (@subst_consn A).
+Proof.
+  intros ? l -> f f' Hff' i.
+  unfold subst_consn. destruct nth_error eqn:Heq; auto.
+Qed.
+
+Instance subst_consn_proper_ext {A} : Proper (Logic.eq ==> `=1` ==> Logic.eq ==> Logic.eq) (@subst_consn A).
+Proof.
+  intros ? l -> f f' Hff' i i' <-.
+  unfold subst_consn. destruct nth_error eqn:Heq; auto.
+Qed.
+
+Fixpoint idsn n : list term :=
+  match n with
+  | 0 => []
+  | S n => idsn n ++ [tRel n]
+  end.
+
+Definition subst_cons_gen {A} (t : A) (f : nat -> A) :=
+  fun i =>
+    match i with
+    | 0 => t
+    | S n => f n
+    end.
+
+Instance subst_cons_gen_proper {A} : Proper (Logic.eq ==> `=1` ==> `=1`) (@subst_cons_gen A).
+Proof. intros x y <- f g Hfg i. destruct i; simpl; auto. Qed.
+
+Lemma subst_consn_subst_cons_gen {A} (t : A) l σ : subst_consn (t :: l) σ =1 (subst_cons_gen t (l ⋅n σ)).
+Proof.
+  intros i. unfold subst_consn. induction i; simpl; trivial.
+Qed.
+
+Lemma subst_consn_app {A} {l l' : list A} {σ} : (l ++ l') ⋅n σ =1 l ⋅n (l' ⋅n σ).
+Proof.
+  induction l; simpl; auto.
+  - now rewrite subst_consn_nil.
+  - now rewrite !subst_consn_subst_cons_gen IHl.
+Qed.
+
+Lemma subst_consn_ge {A} {l : list A} {i σ} : #|l| <= i -> (l ⋅n σ) i = σ (i - #|l|).
+Proof.
+  induction l in i, σ |- *; simpl.
+  - now rewrite subst_consn_nil.
+  - rewrite subst_consn_subst_cons_gen.
+    intros H. destruct i; [lia|]. simpl.
+    apply IHl. lia.
+Qed.
+
+Lemma subst_consn_lt {A} {l : list A} {i} :
+  i < #|l| ->
+  ∑ x, (List.nth_error l i = Some x) /\ (forall σ, (l ⋅n σ) i = x)%type.
+Proof.
+  induction l in i |- *; simpl.
+  - intros H; elimtype False; lia.
+  - intros H.
+    destruct i.
+    + simpl. exists a. split; auto.
+    + specialize (IHl i). forward IHl.
+      * lia.
+      * destruct IHl as [x [Hnth Hsubst_cons]].
+        exists x. simpl. split; auto.
+Qed.
+
+Lemma idsn_length n : #|idsn n| = n.
+Proof.
+  induction n; simpl; auto. rewrite app_length IHn; simpl; lia.
+Qed.
+Hint Rewrite idsn_length : len.
+
+Lemma idsn_lt {n i} : i < n -> nth_error (idsn n) i = Some (tRel i).
+Proof.
+  induction n in i |- *; simpl; auto.
+  - intros H; lia.
+  - intros H. destruct (Compare_dec.le_lt_dec n i).
+    -- assert (n = i) by lia; subst.
+       rewrite nth_error_app_ge idsn_length ?Nat.sub_diag; trea.
+    -- rewrite nth_error_app_lt ?idsn_length //. apply IHn; lia.
+Qed.
+
+Lemma nth_error_idsn_Some :
+  forall n k,
+    k < n ->
+    nth_error (idsn n) k = Some (tRel k).
+Proof.
+  intros n k h.
+  induction n in k, h |- *.
+  - inversion h.
+  - simpl. destruct (Nat.ltb_spec0 k n).
+    + rewrite nth_error_app1.
+      * rewrite idsn_length. auto.
+      * eapply IHn. assumption.
+    + assert (k = n) by lia. subst.
+      rewrite nth_error_app2.
+      * rewrite idsn_length. auto.
+      * rewrite idsn_length. replace (n - n) with 0 by lia.
+        simpl. reflexivity.
+Qed.
+
+Lemma nth_error_idsn_None :
+  forall n k,
+    k >= n ->
+    nth_error (idsn n) k = None.
+Proof.
+  intros n k h.
+  eapply nth_error_None.
+  rewrite idsn_length. auto.
+Qed.
+
+
+Lemma subst_cons_0 t σ : (tRel 0).[t ⋅ σ] = t. Proof. reflexivity. Qed.
+Lemma subst_cons_shift t σ : ↑ ∘s (t ⋅ σ) = σ. Proof. reflexivity. Qed.
+Hint Rewrite subst_cons_0 subst_cons_shift : sigma.
+
+Lemma shiftk_shift n : ↑^(S n) =1 ↑^n ∘s ↑. Proof. reflexivity. Qed.
+
+Lemma shiftk_shift_l n : ↑^(S n) =1 ↑ ∘s ↑^n.
+Proof.
+  intros i.
+  unfold shiftk. unfold subst_compose, shift.
+  simpl. f_equal. lia.
+Qed.
+
+Lemma subst_subst_consn s σ τ : (s ⋅ σ) ∘s τ =1 (s.[τ] ⋅ σ ∘s τ).
+Proof.
+  intros i.
+  destruct i; simpl; reflexivity.
+Qed.
+
+Hint Rewrite subst_subst_consn : sigma.
+
+Definition Upn n σ := idsn n ⋅n (σ ∘s ↑^n).
+Notation "⇑^ n σ" := (Upn n σ) (at level 30, n at level 2, format "⇑^ n  σ") : sigma_scope.
+
+Instance Upn_ext n : Proper (`=1` ==> `=1`) (Upn n).
+Proof.
+  unfold Upn. reduce_goal. now rewrite H.
+Qed.
+
+Lemma Upn_0 σ : ⇑^0 σ =1 σ.
+Proof.
+  unfold Upn. simpl.
+  now rewrite subst_consn_nil shiftk_0 compose_ids_r.
+Qed.
+
+Lemma Upn_1_Up σ : ⇑^1 σ =1 ⇑ σ.
+Proof.
+  unfold Upn.
+  intros i. destruct i; auto.
+  simpl. rewrite subst_consn_ge; simpl; auto with arith.
+Qed.
+Hint Rewrite Upn_1_Up : sigma.
+
+Lemma Upn_eq n σ : Upn n σ = idsn n ⋅n (σ ∘s ↑^n).
+Proof. reflexivity. Qed.
+
+Lemma Upn_proper : Proper (Logic.eq ==> `=1` ==> `=1`) Upn.
+Proof. intros ? ? -> f g Hfg. unfold Upn. now rewrite Hfg. Qed.
+
+(** The σ-calculus equations for Coq *)
+
+Lemma inst_app {s t σ} : (tApp s t).[σ] = tApp s.[σ] t.[σ].
+Proof. reflexivity. Qed.
+
+Lemma inst_lam {na t b σ} : (tLambda na t b).[σ] = tLambda na t.[σ] b.[⇑ σ].
+Proof.
+  simpl. now rewrite up_Up.
+Qed.
+
+Lemma inst_prod {na t b σ} : (tProd na t b).[σ] = tProd na t.[σ] b.[⇑ σ].
+Proof.
+  simpl. now rewrite up_Up.
+Qed.
+
+Lemma inst_letin {na t b b' σ} : (tLetIn na t b b').[σ] = tLetIn na t.[σ] b.[σ] b'.[⇑ σ].
+Proof.
+  simpl. now rewrite up_Up.
+Qed.
+
+Lemma up_Upn {n σ} : up n σ =1 ⇑^n σ.
+Proof.
+  unfold up, Upn.
+  intros i.
+  elim (Nat.leb_spec n i) => H.
+  - rewrite rename_inst.
+    rewrite subst_consn_ge; rewrite idsn_length; auto.
+  - assert (Hle: i < #|idsn n|) by (rewrite idsn_length; lia).
+    edestruct (subst_consn_lt Hle) as [x [Hnth Hsubst_cons]].
+    rewrite Hsubst_cons. rewrite idsn_lt in Hnth; auto. congruence.
+Qed.
+
+Lemma inst_fix {mfix idx σ} : (tFix mfix idx).[σ] =
+                              tFix (map (map_def (inst σ) (inst (⇑^#|mfix| σ))) mfix) idx.
+Proof.
+  simpl. f_equal. apply map_ext. intros x. apply map_def_eq_spec => //.
+  now rewrite up_Upn.
+Qed.
+
+Lemma inst_cofix {mfix idx σ} : (tCoFix mfix idx).[σ] =
+                                tCoFix (map (map_def (inst σ) (inst (⇑^#|mfix| σ))) mfix) idx.
+Proof.
+  simpl. f_equal. apply map_ext. intros x. apply map_def_eq_spec => //.
+  now rewrite up_Upn.
+Qed.
+
+Lemma inst_mkApps :
+  forall t l σ,
+    (mkApps t l).[σ] = mkApps t.[σ] (map (inst σ) l).
+Proof.
+  intros t l σ.
+  induction l in t, σ |- *.
+  - reflexivity.
+  - simpl. rewrite IHl. reflexivity.
+Qed.
+
+Hint Rewrite @inst_app @inst_lam @inst_prod @inst_letin @inst_fix @inst_cofix
+     @inst_mkApps : sigma.
+
+
+Lemma ren_shift : ↑ =1 ren S.
+Proof. reflexivity. Qed.
+
+Lemma compose_ren f g : ren f ∘s ren g =1 ren (g ∘ f).
+Proof.
+  intros i.
+  destruct i; simpl; reflexivity.
+Qed.
+
+Lemma subst_cons_ren i f : (tRel i ⋅ ren f) =1 ren (subst_cons_gen i f).
+Proof.
+  intros x; destruct x; auto.
+Qed.
+
+Fixpoint ren_ids (n : nat) :=
+  match n with
+  | 0 => []
+  | S n => ren_ids n ++ [n]
+  end.
+
+Lemma ren_ids_length n : #|ren_ids n| = n.
+Proof. induction n; simpl; auto. rewrite app_length IHn; simpl; lia. Qed.
+
+Lemma ren_ids_lt {n i} : i < n -> nth_error (ren_ids n) i = Some i.
+Proof.
+  induction n in i |- *; simpl; auto.
+  - intros H; lia.
+  - intros H. destruct (Compare_dec.le_lt_dec n i).
+    -- assert (n = i) by lia; subst.
+       rewrite nth_error_app_ge ren_ids_length ?Nat.sub_diag; trea.
+    -- rewrite nth_error_app_lt ?ren_ids_length //. apply IHn; lia.
+Qed.
+
+Infix "=2" := (Logic.eq ==> (pointwise_relation _ Logic.eq))%signature (at level 80).
+
+Definition compose2 {A B C} (g : B -> C) (f : A -> B) : A -> C :=
+  fun x => g (f x).
+Infix "∘'" := compose2 (at level 90).
+
+Delimit Scope program_scope with prog.
+
+Lemma subst_consn_subst_cons' {A} (t : A) l : subst_consn (t :: l) =2 ((subst_cons_gen t) ∘ (subst_consn l)).
+Proof. red.
+  intros x y <-. apply subst_consn_subst_cons_gen.
+Qed.
+
+Lemma subst_consn_ids_ren n f : (idsn n ⋅n ren f) =1 ren (ren_ids n ⋅n f).
+Proof.
+  intros i.
+  destruct (Nat.leb_spec n i).
+  - rewrite subst_consn_ge idsn_length; auto.
+    unfold ren. f_equal. rewrite subst_consn_ge ren_ids_length; auto.
+  - assert (Hr:i < #|ren_ids n|) by (rewrite ren_ids_length; lia).
+    assert (Hi:i < #|idsn n|) by (rewrite idsn_length; lia).
+    destruct (subst_consn_lt Hi) as [x' [Hnth He]].
+    destruct (subst_consn_lt Hr) as [x'' [Hnth' He']].
+    rewrite (idsn_lt H) in Hnth.
+    rewrite (ren_ids_lt H) in Hnth'.
+    injection Hnth as <-. injection Hnth' as <-. rewrite He.
+    unfold ren. now rewrite He'.
+Qed.
+
+Lemma ren_shiftk n : ↑^n =1 ren (Nat.add n).
+Proof. reflexivity. Qed.
+
+(** Specific lemma for the fix/cofix cases where we are subst_cons'ing a list of ids in front
+    of the substitution. *)
+Lemma ren_subst_consn_comm:
+  forall (f : nat -> nat) (σ : nat -> term) (n : nat),
+    ren (subst_consn (ren_ids n) (Init.Nat.add n ∘ f)) ∘s subst_consn (idsn n) (σ ∘s ↑^n) =1
+    subst_consn (idsn n) (ren f ∘s σ ∘s ↑^n).
+Proof.
+  intros f σ m i.
+  destruct (Nat.leb_spec m i).
+  -- unfold ren, subst_compose. simpl.
+     rewrite [subst_consn (idsn _) _ i]subst_consn_ge ?idsn_length; try lia.
+     rewrite [subst_consn (ren_ids _) _ i]subst_consn_ge ?ren_ids_length; try lia.
+     rewrite subst_consn_ge ?idsn_length; lia_f_equal.
+  -- assert (Hr:i < #|ren_ids m |) by (rewrite ren_ids_length; lia).
+     assert (Hi:i < #|idsn m |) by (rewrite idsn_length; lia).
+     destruct (subst_consn_lt Hi) as [x' [Hnth He]].
+     rewrite He.
+     unfold ren, subst_compose. simpl.
+     destruct (subst_consn_lt Hr) as [x'' [Hnth' He']].
+     rewrite He'. rewrite (idsn_lt H) in Hnth. injection Hnth as <-.
+     rewrite (ren_ids_lt H) in Hnth'. injection Hnth' as <-.
+     rewrite He. reflexivity.
+Qed.
+
+(** Simplify away iterated up's *)
+Hint Rewrite @up_Upn : sigma.
+
+Lemma rename_inst_assoc t f σ : t.[ren f].[σ] = t.[ren f ∘s σ].
+Proof.
+  revert f σ.
+  elim t using term_forall_list_ind; simpl in |- *; intros; try easy ;
+    try (try rewrite H; try rewrite H0 ; try rewrite H1 ; easy);
+    try solve [f_equal; solve_all].
+
+  - f_equal. rewrite map_map_compose; solve_all.
+  - f_equal; auto. sigma.
+    unfold Up.
+    simpl. rewrite ren_shift. rewrite compose_ren subst_cons_ren H0.
+    apply inst_ext. intros i. destruct i; auto.
+  - f_equal; auto. sigma.
+    unfold Up.
+    rewrite ren_shift. rewrite compose_ren subst_cons_ren H0.
+    apply inst_ext. intros i. destruct i; auto.
+  - f_equal; auto. sigma.
+    unfold Up.
+    rewrite ren_shift. rewrite compose_ren subst_cons_ren H1.
+    apply inst_ext. intros i. destruct i; auto.
+  - f_equal; auto; solve_all; sigma.
+    * rewrite map_predicate_map_predicate; solve_all.
+      rewrite !ren_shiftn e -ren_shiftn.
+      rewrite !up_Upn. unfold Upn.
+      rewrite !compose_ren !subst_consn_ids_ren.
+      apply inst_ext. apply ren_subst_consn_comm.
+    * rewrite map_map_compose. solve_all.
+      rewrite map_branch_map_branch. apply map_branch_eq_spec.
+      sigma.
+      unfold Upn. rewrite !compose_ren !subst_consn_ids_ren H0.
+      apply inst_ext, ren_subst_consn_comm.
+  - f_equal; auto.
+    red in X. rewrite map_map_compose. solve_all.
+    rewrite map_def_map_def map_length. apply map_def_eq_spec; solve_all.
+    sigma.
+    unfold Upn. rewrite !compose_ren.
+    rewrite !subst_consn_ids_ren.
+    rewrite b. simpl. apply inst_ext. apply ren_subst_consn_comm.
+  - f_equal; auto.
+    red in X. rewrite map_map_compose. solve_all.
+    rewrite map_def_map_def map_length. apply map_def_eq_spec; solve_all.
+    sigma.
+    unfold Upn. rewrite !compose_ren.
+    rewrite !subst_consn_ids_ren.
+    rewrite b. simpl. apply inst_ext, ren_subst_consn_comm.
+Qed.
+
+Lemma inst_rename_assoc_n:
+  forall (f : nat -> nat) (σ : nat -> term) (n : nat),
+    subst_consn (idsn n) (σ ∘s ↑^n) ∘s ren (subst_consn (ren_ids n) (Init.Nat.add n ∘ f)) =1
+    subst_consn (idsn n) (σ ∘s ren f ∘s ↑^n).
+Proof.
+  intros f σ m. rewrite ren_shiftk.
+  intros i.
+  destruct (Nat.leb_spec m i).
+  -- rewrite [subst_consn (idsn _) _ i]subst_consn_ge ?idsn_length; try lia.
+     unfold subst_compose.
+     rewrite [subst_consn (idsn _) _ i]subst_consn_ge ?idsn_length; try lia.
+     rewrite !rename_inst_assoc !compose_ren.
+     apply inst_ext. intros i'.
+     unfold ren. f_equal. rewrite subst_consn_ge ?ren_ids_length; try lia.
+     now assert (m + i' - m = i') as -> by lia.
+  -- assert (Hr:i < #|ren_ids m |) by (rewrite ren_ids_length; lia).
+     assert (Hi:i < #|idsn m |) by (rewrite idsn_length; lia).
+     destruct (subst_consn_lt Hi) as [x' [Hnth He]].
+     rewrite He.
+     unfold subst_compose. simpl.
+     rewrite (idsn_lt H) in Hnth. injection Hnth as <-. rewrite He.
+     simpl. unfold ren. f_equal.
+     destruct (subst_consn_lt Hr) as [x'' [Hnth' He']].
+     rewrite (ren_ids_lt H) in Hnth'. injection Hnth' as <-. now rewrite He'.
+Qed.
+
+Lemma inst_rename_assoc t f σ : t.[σ].[ren f] = t.[σ ∘s ren f].
+Proof.
+  revert f σ.
+  elim t using term_forall_list_ind; simpl in |- *; intros; try easy ;
+    try (try rewrite H; try rewrite H0 ; try rewrite H1 ; easy);
+    try solve [f_equal; solve_all].
+
+  - f_equal. rewrite map_map_compose; solve_all.
+  - f_equal; auto. sigma.
+    unfold Up.
+    rewrite ren_shift. rewrite compose_ren subst_cons_ren H0.
+    apply inst_ext. intros i. destruct i; auto. simpl.
+    unfold subst_compose. simpl. now rewrite !rename_inst_assoc !compose_ren.
+  - f_equal; auto. sigma.
+    unfold Up.
+    rewrite ren_shift. rewrite compose_ren subst_cons_ren H0.
+    apply inst_ext. intros i. destruct i; auto.
+    unfold subst_compose. simpl. now rewrite !rename_inst_assoc !compose_ren.
+  - f_equal; auto. sigma.
+    unfold Up.
+    rewrite ren_shift. rewrite compose_ren subst_cons_ren H1.
+    apply inst_ext. intros i. destruct i; auto.
+    unfold subst_compose. simpl. now rewrite !rename_inst_assoc !compose_ren.
+  - f_equal; auto; solve_all; sigma.
+    * rewrite map_predicate_map_predicate. apply map_predicate_eq_spec => //.
+      + solve_all.
+      + rewrite !up_Upn. unfold Upn; rewrite !compose_ren subst_consn_ids_ren e /=.
+        apply inst_ext, inst_rename_assoc_n.
+    * rewrite map_map_compose; solve_all; rewrite map_branch_map_branch; 
+      apply map_branch_eq_spec. sigma.
+      unfold Upn; rewrite !compose_ren subst_consn_ids_ren H0 /=.
+      apply inst_ext, inst_rename_assoc_n.
+  - f_equal; auto.
+    red in X. rewrite map_map_compose. solve_all.
+    rewrite map_def_map_def map_length. apply map_def_eq_spec; solve_all.
+    sigma.
+    unfold Upn. rewrite !compose_ren.
+    rewrite !subst_consn_ids_ren.
+    rewrite b. simpl. apply inst_ext. apply inst_rename_assoc_n.
+  - f_equal; auto.
+    red in X. rewrite map_map_compose. solve_all.
+    rewrite map_def_map_def map_length. apply map_def_eq_spec; solve_all.
+    sigma.
+    unfold Upn. rewrite !compose_ren.
+    rewrite !subst_consn_ids_ren.
+    rewrite b. simpl. apply inst_ext, inst_rename_assoc_n.
+Qed.
+
+Lemma rename_subst_compose1 r s s' : ren r ∘s (s ∘s s') =1 ren r ∘s s ∘s s'.
+Proof. unfold subst_compose. simpl. intros i. reflexivity. Qed.
+
+Lemma rename_subst_compose2 r s s' : s ∘s (ren r ∘s s') =1 s ∘s ren r ∘s s'.
+Proof.
+  unfold subst_compose. simpl. intros i.
+  rewrite rename_inst_assoc. reflexivity.
+Qed.
+
+Lemma rename_subst_compose3 r s s' : s ∘s (s' ∘s ren r) =1 s ∘s s' ∘s ren r.
+Proof.
+  unfold subst_compose. simpl. intros i.
+  rewrite inst_rename_assoc. reflexivity.
+Qed.
+
+Lemma Up_Up_assoc:
+  forall s s' : nat -> term, (⇑ s) ∘s (⇑ s') =1 ⇑ (s ∘s s').
+Proof.
+  intros s s'.
+  unfold Up.
+  rewrite ren_shift.
+  rewrite subst_subst_consn.
+  simpl. apply subst_cons_proper => //.
+  rewrite - rename_subst_compose2.
+  rewrite - rename_subst_compose3.
+  now apply subst_compose_proper; auto.
+Qed.
+
+Hint Rewrite Up_Up_assoc : sigma.
+
+Lemma up_up_assoc:
+  forall (s s' : nat -> term) (n : nat), up n s ∘s up n s' =1 up n (s ∘s s').
+Proof.
+  intros s s' n i.
+  unfold up, subst_compose. simpl.
+  destruct (Nat.leb_spec n i).
+  - rewrite !(rename_inst (Nat.add n) (s (i - n))).
+    rewrite rename_inst_assoc.
+    rewrite !(rename_inst (Nat.add n) _).
+    rewrite inst_rename_assoc.
+    apply inst_ext.
+    intros i'. unfold subst_compose.
+    unfold ren. simpl.
+    destruct (Nat.leb_spec n (n + i')).
+    * rewrite rename_inst.
+      now assert (n + i' - n = i') as -> by lia.
+    * lia.
+  - simpl.
+    destruct (Nat.leb_spec n i); lia_f_equal.
+Qed.
+
+Lemma inst_assoc t s s' : t.[s].[s'] = t.[s ∘s s'].
+Proof.
+  revert s s'.
+  elim t using term_forall_list_ind; simpl in |- *; intros; try easy ;
+    try (try rewrite H; try rewrite H0 ; try rewrite H1 ; easy);
+    try solve [f_equal; solve_all].
+
+  - f_equal. rewrite map_map_compose; solve_all.
+  - f_equal; auto. sigma.
+    now rewrite H0 Up_Up_assoc.
+  - f_equal; auto. sigma.
+    now rewrite H0 Up_Up_assoc.
+  - f_equal; auto. sigma.
+    now rewrite H1 Up_Up_assoc.
+  - f_equal; auto.
+    * rewrite map_predicate_map_predicate; solve_all.
+      now rewrite e up_up_assoc.
+    * rewrite map_map_compose; solve_all.
+      rewrite map_branch_map_branch. apply map_branch_eq_spec; solve_all.
+      now rewrite H0 up_up_assoc.
+  - f_equal; auto. sigma.
+    rewrite map_map_compose; solve_all.
+    rewrite map_def_map_def.
+    apply map_def_eq_spec; auto.
+    rewrite b.
+    now rewrite map_length up_up_assoc.
+  - f_equal; auto. sigma.
+    rewrite map_map_compose; solve_all.
+    rewrite map_def_map_def.
+    apply map_def_eq_spec; auto.
+    rewrite b.
+    now rewrite map_length up_up_assoc.
+Qed.
+
+Hint Rewrite inst_assoc : sigma.
+
+Lemma subst_compose_assoc s s' s'' : (s ∘s s') ∘s s'' =1 s ∘s (s' ∘s s'').
+Proof.
+  intros i; unfold subst_compose at 1 3 4.
+  now rewrite inst_assoc.
+Qed.
+
+Hint Rewrite subst_compose_assoc : sigma.
+
+Lemma subst_cons_0_shift : (tRel 0 ⋅ ↑) =1 ids.
+Proof. intros i. destruct i; reflexivity. Qed.
+
+Hint Rewrite subst_cons_0_shift : sigma.
+
+Lemma subst_cons_0s_shifts σ : ((σ 0) ⋅ (↑ ∘s σ)) =1 σ.
+Proof.
+  intros i. destruct i; auto.
+Qed.
+
+Hint Rewrite subst_cons_0s_shifts : sigma.
+
+Lemma Upn_Up σ n : ⇑^(S n) σ =1 ⇑^n ⇑ σ.
+Proof.
+  intros i. unfold Upn.
+  simpl. rewrite subst_consn_app.
+  rewrite subst_consn_tip. unfold Up. apply subst_consn_proper; auto.
+  rewrite shiftk_shift_l.
+  intros i'. unfold subst_cons, subst_compose.
+  destruct i' => //; auto; simpl. 
+  - unfold shiftk. now rewrite Nat.add_0_r.
+  - simpl. now rewrite inst_assoc.
+Qed.
+
+Lemma Upn_1 σ : ⇑^1 σ =1 ⇑ σ.
+Proof. now rewrite Upn_Up Upn_0. Qed.
+
+Lemma Upn_S σ n : ⇑^(S n) σ =1 ⇑ ⇑^n σ.
+Proof.
+  rewrite Upn_Up. induction n in σ |- *.
+  * rewrite !Upn_0. now eapply Up_ext.
+  * rewrite Upn_Up. rewrite IHn. eapply Up_ext. now rewrite Upn_Up.
+Qed.
+Hint Rewrite Upn_0 Upn_S : sigma.
+
+(* Print Rewrite HintDb sigma. *)
+
+Lemma subst_inst_aux s k t : subst s k t = inst (up k (subst_fn s)) t.
+Proof.
+  revert s k.
+  elim t using term_forall_list_ind; simpl in |- *; intros; try easy ;
+    try (try rewrite H; try rewrite H0 ; try rewrite H1 ; easy);
+    try solve [f_equal; solve_all].
+
+  - unfold subst_fn, up.
+    elim (Nat.leb_spec k n) => //.
+    intros H.
+    destruct nth_error eqn:Heq.
+    * apply lift_rename.
+    * simpl. eapply nth_error_None in Heq. lia_f_equal.
+  - f_equal; eauto.
+    rewrite H0. apply inst_ext. intros t'; now rewrite (up_up 1 k).
+  - f_equal; eauto.
+    rewrite H0. apply inst_ext. intros t'; now rewrite (up_up 1 k).
+  - f_equal; eauto.
+    rewrite H1. apply inst_ext. intros t'; now rewrite (up_up 1 k).
+  - f_equal; eauto.
+    * apply map_predicate_eq_spec; auto; solve_all.
+      rewrite e. now rewrite (up_up #|pcontext p| k).
+    * solve_all. apply map_branch_eq_spec.
+      now rewrite (up_up #|bcontext x| k).
+  - f_equal; eauto; solve_all; auto. apply map_def_eq_spec; auto.
+    rewrite b. apply inst_ext. intros t'; now rewrite (up_up #|m| k).
+  - f_equal; eauto.
+    solve_all; auto. apply map_def_eq_spec; auto.
+    rewrite b. apply inst_ext. intros t'; now rewrite (up_up #|m| k).
+Qed.
+
+Lemma subst_fn_subst_consn s : subst_fn s =1 subst_consn s ids.
+Proof. reflexivity. Qed.
+
+Theorem subst_inst s k t : subst s k t = inst (⇑^k (subst_consn s ids)) t.
+Proof.
+  rewrite subst_inst_aux up_Upn. apply inst_ext.
+  unfold Upn. now rewrite subst_fn_subst_consn.
+Qed.
+
+(** Simplify away [subst] to the σ-calculus [inst] primitive. *)
+Hint Rewrite @subst_inst : sigma.
+Hint Rewrite @subst_consn_nil : sigma.
+
+Hint Rewrite shiftk_shift_l shiftk_shift : sigma.
+(* Hint Rewrite Upn_eq : sigma. *)
+
+
+Fixpoint subst_app (t : term) (us : list term) : term :=
+  match t, us with
+  | tLambda _ A t, u :: us => subst_app (t {0 := u}) us
+  | _, [] => t
+  | _, _ => mkApps t us
+  end.
 
 Lemma shiftn0 r : shiftn 0 r =1 r.
 Proof.
@@ -43,11 +1045,11 @@ Qed.
 
 Lemma subst_consn_shiftn n (l : list term) σ : #|l| = n -> ↑^n ∘s (l ⋅n σ) =1 σ.
 Proof.
-  induction n in l |- *; simpl; intros; autorewrite with sigma.
-  - destruct l; try discriminate. simpl; autorewrite with sigma. reflexivity.
+  induction n in l |- *; simpl; intros; sigma.
+  - destruct l; try discriminate. now sigma. 
   - destruct l; try discriminate. simpl in *.
     rewrite subst_consn_subst_cons.
-    simpl; autorewrite with sigma. apply IHn. lia.
+    simpl; sigma. apply IHn. lia.
 Qed.
 
 Lemma shiftn_consn_idsn n σ : ↑^n ∘s ⇑^n σ =1 σ ∘s ↑^n.
@@ -55,7 +1057,7 @@ Proof.
   unfold Upn. rewrite subst_consn_shiftn; [reflexivity|].
   now rewrite idsn_length.
 Qed.
-Hint Rewrite shiftn_consn_idsn: sigma.
+(* Hint Rewrite shiftn_consn_idsn: sigma. *)
 
 Lemma subst_consn_compose l σ' σ : l ⋅n σ' ∘s σ =1 (map (inst σ) l ⋅n (σ' ∘s σ)).
 Proof.
@@ -123,12 +1125,19 @@ Proof.
     now rewrite subst_compose_assoc IHn -shiftk_shift shiftk_shift_l.
 Qed.
 
+Lemma Upn_Upn k k' σ : ⇑^(k + k') σ =1 ⇑^k (⇑^k' σ).
+Proof.
+  setoid_rewrite <- up_Upn. rewrite -(@up_Upn k').
+  symmetry; apply up_up.
+Qed.
+Hint Rewrite Upn_Upn : sigma.
+
 Lemma Upn_compose n σ σ' : ⇑^n σ ∘s ⇑^n σ' =1 ⇑^n (σ ∘s σ').
 Proof.
   induction n.
   - unfold Upn. simpl.
     now rewrite !subst_consn_nil !shiftk_0 !compose_ids_r.
-  - rewrite !Upn_S. autorewrite with sigma. now rewrite IHn.
+  - setoid_rewrite Upn_S. sigma. now rewrite IHn.
 Qed.
 
 Lemma up_ext_closed k' k s s' :
@@ -159,7 +1168,7 @@ Proof.
   intros u t k.
   induction t in k |- * using term_forall_list_ind.
   all: simpl. all: auto.
-  all: autorewrite with sigma.
+  all: sigma.
   all: rewrite ?map_map_compose ?compose_on_snd ?compose_map_def ?map_length 
     ?map_predicate_map_predicate ?map_branch_map_branch; unfold map_branch.
   all: try solve [ f_equal ; eauto ; solve_all ; eauto ].
@@ -169,15 +1178,19 @@ Proof.
       reflexivity.
     + rewrite nth_error_idsn_None. 1: lia.
       reflexivity.
-  - rewrite IHt1. specialize (IHt2 (S k)). autorewrite with sigma in IHt2.
+  - rewrite IHt1. specialize (IHt2 (S k)).
+    setoid_rewrite Upn_S in IHt2.
     rewrite IHt2. reflexivity.
-  - rewrite IHt1. specialize (IHt2 (S k)). autorewrite with sigma in IHt2.
+  - rewrite IHt1. specialize (IHt2 (S k)).
+    setoid_rewrite Upn_S in IHt2.
     rewrite IHt2. reflexivity.
-  - rewrite IHt1 IHt2. specialize (IHt3 (S k)). autorewrite with sigma in IHt3.
+  - rewrite IHt1 IHt2. specialize (IHt3 (S k)).
+    setoid_rewrite Upn_S in IHt3.
     rewrite IHt3. reflexivity.
   - f_equal.
-    * destruct X. solve_all.
-      now rewrite -Upn_Upn e.
+    * destruct X. solve_all. sigma.
+      setoid_rewrite <-Upn_Upn.
+      now rewrite e.
     * apply IHt.
     * solve_all. f_equal.
       now rewrite up_Upn -Upn_Upn H.
@@ -188,7 +1201,7 @@ Proof.
     apply map_def_eq_spec. 
     * apply IH.
     * specialize (IH' (#|m| + k)).
-      autorewrite with sigma.
+      sigma.
       now rewrite - !up_Upn up_up !up_Upn.
   - f_equal.
     autorewrite with len.
@@ -210,26 +1223,6 @@ Proof.
   - destruct (Nat.ltb_spec i (n + m)); try lia;
     destruct (Nat.ltb_spec (i - n) m); try lia.
     rewrite Nat.add_assoc. f_equal. f_equal. lia.  
-Qed.
-
-Ltac nat_compare_specs :=
-  match goal with
-  | |- context [?x <=? ?y] =>
-    destruct (Nat.leb_spec x y); try lia
-  | |- context [?x <? ?y] =>
-    destruct (Nat.ltb_spec x y); try lia
-  end.
-
-Instance shiftn_proper : Proper (Logic.eq ==> `=1` ==> `=1`) shiftn.
-Proof.
-  intros x y -> f g Hfg.
-  unfold shiftn; intros i.
-  nat_compare_specs. now rewrite Hfg.
-Qed.
-
-Instance map_decl_proper : Proper (`=1` ==> Logic.eq ==> Logic.eq) map_decl.
-Proof.
-  intros f g Hfg x y ->. now apply map_decl_ext.
 Qed.
 
 Lemma nth_error_idsn_eq_Some n k i : nth_error (idsn n) k = Some i -> i = tRel k.
